theories/proofmode/coq_tactics.v
@@ -1325,19 +1325,24 @@ Implicit Types Δ : envs PROP.
 Implicit Types P Q : PROP.
 
 (** * Invariants *)
-Lemma tac_inv_elim Δ Δ' i j φ p Pinv Pin Pout (Pclose : option PROP) Q Q' :
+Lemma tac_inv_elim {X : Type} Δ Δ' i j φ p Pinv Pin Pout (Pclose : option (X → PROP))
+      Q (Q' : X → PROP) :
   envs_lookup_delete false i Δ = Some (p, Pinv, Δ') →
   ElimInv φ Pinv Pin Pout Pclose Q Q' →
   φ →
   (∀ R, ∃ Δ'',
-    envs_app false (Esnoc Enil j (Pin -∗ (Pout -∗ maybe_wand Pclose Q') -∗ R)%I) Δ' = Some Δ'' ∧
+    envs_app false (Esnoc Enil j
+                    (Pin -∗ (∀ x, Pout x -∗ default (Q' x) Pclose (λ Pclose, Pclose x -∗ Q' x)) -∗ R)%I) Δ'
+      = Some Δ'' ∧
     envs_entails Δ'' R) →
   envs_entails Δ Q.
 Proof.
-  rewrite envs_entails_eq=> /envs_lookup_delete_Some [? ->] ?? /(_ Q) [Δ'' [? <-]].
+  rewrite envs_entails_eq=> /envs_lookup_delete_Some [? ->] Hinv ? /(_ Q) [Δ'' [? <-]].
   rewrite (envs_lookup_sound' _ false) // envs_app_singleton_sound //; simpl.
   apply wand_elim_r', wand_mono; last done. apply wand_intro_r, wand_intro_r.
-  rewrite intuitionistically_if_elim maybe_wand_sound -assoc wand_curry. auto.
+  rewrite intuitionistically_if_elim -assoc. destruct Pclose; simpl in *.
+  - setoid_rewrite wand_curry. auto.
+  - setoid_rewrite <-(right_id emp%I _ (Pout _)). auto.
 Qed.
 
 (** * Rewriting *)
