theories/proofmode/monpred.v
@@ -486,21 +486,28 @@ Global Instance add_modal_at_fupd_goal `{BiFUpd PROP} E1 E2 𝓟 𝓟' Q i :
   AddModal 𝓟 𝓟' (|={E1,E2}=> Q i) → AddModal 𝓟 𝓟' ((|={E1,E2}=> Q) i).
 Proof. by rewrite /AddModal !monPred_at_fupd. Qed.
 
-Global Instance elim_inv_embed_with_close φ 𝓟inv 𝓟in 𝓟out 𝓟close Pin Pout Pclose Q Q' :
-  (∀ i, ElimInv φ 𝓟inv 𝓟in 𝓟out (Some 𝓟close) (Q i) (Q' i)) →
-  MakeEmbed 𝓟in Pin → MakeEmbed 𝓟out Pout → MakeEmbed 𝓟close Pclose →
-  ElimInv φ ⎡𝓟inv⎤ Pin Pout (Some Pclose) Q Q'.
+Global Instance elim_inv_embed_with_close {X : Type} φ
+       𝓟inv 𝓟in (𝓟out 𝓟close : X → PROP)
+       Pin (Pout Pclose : X → monPred)
+       Q (Q' : X → monPred) :
+  (∀ i, ElimInv φ 𝓟inv 𝓟in 𝓟out (Some 𝓟close) (Q i) (λ x, Q' x i)) →
+  MakeEmbed 𝓟in Pin → (∀ x, MakeEmbed (𝓟out x) (Pout x)) →
+  (∀ x, MakeEmbed (𝓟close x) (Pclose x)) →
+  ElimInv (X:=X) φ ⎡𝓟inv⎤ Pin Pout (Some Pclose) Q Q'.
 Proof.
-  rewrite /MakeEmbed /ElimInv=>H <- <- <- ?. iStartProof PROP.
-  iIntros (?) "(?&?&HQ')". iApply H; [done|]. iFrame. iIntros "?". by iApply "HQ'".
+  rewrite /MakeEmbed /ElimInv=>H <- Hout Hclose ?. iStartProof PROP.
+  setoid_rewrite <-Hout. setoid_rewrite <-Hclose.
+  iIntros (?) "(?&?&HQ')". iApply H; [done|]. iFrame. iIntros (x) "?". by iApply "HQ'".
 Qed.
-Global Instance elim_inv_embed_without_close φ 𝓟inv 𝓟in 𝓟out Pin Pout Q Q' :
-  (∀ i, ElimInv φ 𝓟inv 𝓟in 𝓟out None (Q i) (Q' i)) →
-  MakeEmbed 𝓟in Pin → MakeEmbed 𝓟out Pout →
-  ElimInv φ ⎡𝓟inv⎤ Pin Pout None Q Q'.
+Global Instance elim_inv_embed_without_close  {X : Type}
+       φ 𝓟inv 𝓟in (𝓟out : X → PROP) Pin (Pout : X → monPred) Q (Q' : X → monPred) :
+  (∀ i, ElimInv φ 𝓟inv 𝓟in 𝓟out None (Q i) (λ x, Q' x i)) →
+  MakeEmbed 𝓟in Pin → (∀ x, MakeEmbed (𝓟out x) (Pout x)) →
+  ElimInv (X:=X) φ ⎡𝓟inv⎤ Pin Pout None Q Q'.
 Proof.
-  rewrite /MakeEmbed /ElimInv=>H <- <- ?. iStartProof PROP.
-  iIntros (?) "(?&?&HQ')". iApply H; [done|]. iFrame. iIntros "?". by iApply "HQ'".
+  rewrite /MakeEmbed /ElimInv=>H <-Hout ?. iStartProof PROP.
+  setoid_rewrite <-Hout.
+  iIntros (?) "(?&?&HQ')". iApply H; [done|]. iFrame. iIntros (x) "?". by iApply "HQ'".
 Qed.
 
 End sbi.
